```js
var decode = function(encoded) {
    const n = encoded.length+1
    let all = 0
    for (let num = 1; num <= n; num++) all ^= num
    let _1Ton_1 = 0
    for (let i = 1; i < encoded.length; i+=2) {
        _1Ton_1 ^= encoded[i]
    }
    let perm = [all^_1Ton_1]
    for (let i = 0; i < encoded.length; i++) {
        perm[i+1] = perm[i]^encoded[i]
    }
    return perm
};
```

思路：已知

```js
encoded[1] = perm[1]^perm[2]
encoded[3] = perm[3]^perm[4]
...
encoded[n-2] = perm[n-2]^perm[n-1]
```

令`_1Ton_1 = encoded[1]^encoded[3]^...^encoded[n-2] = perm[1]^perm[2]^perm[3]^...^perm[n-1]`，

令`all = 1^2^3^...^n = perm[0]^perm[1]^...^perm[n-1]`，

于是有`perm[0] = _1Ton_1^all`。